theories/Universe.v
@@ -1,7 +1,18 @@
 Class Universe := {
-  event: Type;
+  syscall: Type;
   val: Type;
 }
 .
 
 Context `{Universe}.
+
+Inductive event: Type :=
+| event_sys
+    (sys: syscall)
+| event_exit (rv: val)
+(* | event_tau *)
+| event_ub
+| event_nb
+.
+
+(* Coercion event_sys: syscall >-> event. *)
