theories/Behavior.v
@@ -1,0 +1,116 @@
+Require Import sflib.
+Require Import Universe.
+Require Import Semantics.
+From Paco Require Import paco.
+Require Import RelationClasses List.
+Require Import ClassicalChoice PropExtensionality FunctionalExtensionality.
+(* Require Import Streams. *)
+
+Ltac et := eauto.
+
+Module Beh.
+  CoInductive t: Type :=
+  | done
+  | spin
+  | cons (hd: event) (tl: t)
+  .
+  Infix "##" := cons (at level 60, right associativity).
+  (*** past -------------> future ***)
+  (*** a ## b ## c ## spin / done ***)
+
+  (*** le src tgt ***)
+  Inductive _le (le: t -> t -> Prop): t -> t -> Prop :=
+  | le_done
+    :
+      _le le (done) (done)
+  | le_ub
+      tl beh
+    :
+      _le le (event_ub ## tl) beh
+  | le_nb
+      tl beh
+    :
+      _le le beh (event_nb ## tl)
+  | le_step
+      ev tl0 tl1
+      (TL: le tl0 tl1)
+    :
+      _le le (ev ## tl0) (ev ## tl1)
+  .
+
+  Definition le: _ -> _ -> Prop := paco2 _le bot2.
+
+  Lemma le_mon: monotone2 _le.
+  Proof.
+    ii. inv IN; econs; eauto.
+  Qed.
+
+  Hint Constructors _le.
+  Hint Unfold le.
+  Hint Resolve le_mon: paco.
+
+  Remark ub_test ev: le (event_ub ## done) (ev ## done). pfold. econs; eauto. Qed.
+  Remark ub_prefix s0: ~ le ((event_sys s0) ## event_ub ## done) done. ii. punfold H. inv H. Qed.
+
+End Beh.
+
+
+
+Section BEHAVES.
+
+Variable L: semantics.
+
+Definition union (st0: L.(state)) (P: (option event) -> L.(state) -> Prop) :=
+  exists ev st1, <<STEP: L.(step) st0 ev st1>> /\ <<UNION: P ev st1>>.
+Definition inter (st0: L.(state)) (P: (option event) -> L.(state) -> Prop) :=
+  forall ev st1 (STEP: L.(step) st0 ev st1), <<INTER: P ev st1>>.
+
+Inductive _state_behaves (state_behaves: L.(state) -> Beh.t -> Prop)
+          (st0: L.(state)): Beh.t -> Prop :=
+| sb_final
+    (FINAL: L.(state_sort) st0 = final)
+  :
+    _state_behaves state_behaves st0 (Beh.done)
+| sb_angelic
+    ev evs
+    (ANG: L.(state_sort) st0 = angelic)
+    (STEP: inter st0 (fun e st1 => <<TL: state_behaves st1 evs>> /\ <<HD: e = Some ev>>))
+  :
+    _state_behaves state_behaves st0 (Beh.cons ev evs)
+| sb_demonic
+    ev evs
+    (DEM: L.(state_sort) st0 = demonic)
+    (STEP: union st0 (fun e st1 => <<TL: state_behaves st1 evs>> /\ <<HD: e = Some ev>>))
+  :
+    _state_behaves state_behaves st0 (Beh.cons ev evs)
+| sb_angelic_spin
+    (ANG: L.(state_sort) st0 = angelic)
+    (STEP: inter st0 (fun e st1 => <<TL: state_behaves st1 Beh.spin>> /\ <<HD: e = None>>))
+  :
+    _state_behaves state_behaves st0 Beh.spin 
+| sb_demonic_spin
+    (ANG: L.(state_sort) st0 = demonic)
+    (STEP: union st0 (fun e st1 => <<TL: state_behaves st1 Beh.spin>> /\ <<HD: e = None>>))
+  :
+    _state_behaves state_behaves st0 Beh.spin 
+.
+
+Definition state_behaves: _ -> _ -> Prop := paco2 _state_behaves bot2.
+
+Lemma state_behaves_mon: monotone2 _state_behaves.
+Proof.
+  ii. inv IN.
+  - econs; eauto.
+  - econs 2; eauto. ii. exploit STEP; et. i; des. eauto.
+  - econs 3; eauto. rr in STEP. des. rr. esplits; eauto.
+  - econs 4; eauto. ii. exploit STEP; et. i; des. eauto.
+  - econs 5; eauto. rr in STEP. des. rr. esplits; eauto.
+Qed.
+
+Hint Constructors _state_behaves.
+Hint Unfold state_behaves.
+Hint Resolve state_behaves_mon: paco.
+
+Definition program_behaves: behavior -> Prop := state_behaves L.(initial_state).
+
+End BEHAVES.
